transitivity proof sketch

subtyping/subtyping.v
@@ -2,7 +2,7 @@ Require Import ST.src.stream ST.src.st ST.src.so ST.src.si ST.src.reordering
                ST.src.siso ST.types.local ST.subtyping.refinement ST.src.reorderingfacts.
 From mathcomp Require Import all_ssreflect seq ssrnat.
 From Paco Require Import paco.
-Require Import String List Coq.Arith.Even.
+Require Import String List.
 Import ListNotations.
 Require Import Setoid.
 Require Import Morphisms.
@@ -33,4 +33,302 @@ Definition subtype2 (T T': st): Prop := exists (l: list (siso*siso)), decomposeL
 Definition subltype (T T': local) (T1 T2: st) (P: lt2stC T T1) (Q: lt2stC T' T2) := subtype T1 T2.
 
 Definition subltype2 (T T': local) (T1 T2: st) (P: lt2stC T T1) (Q: lt2stC T' T2) := subtype2 T1 T2.
+
+Lemma pneqq: forall p q a l l' s s' w w' (H: p <> q),
+  q & [(l, s, w)] = merge_ap_cont p (ap_merge q H p s a) (p & [(l', s', w')]) ->
+  w = merge_ap_cont p a (p & [(l', s', w')]) .
+Proof. intros p q a.
+       induction a; intros.
+       - rewrite(st_eq( merge_ap_cont p (ap_merge q H p s1 (ap_receive q0 n s s0)) (p & [(l', s', w')]))) in H0.
+         simpl in H0. inversion H0. subst. easy.
+       - rewrite(st_eq(merge_ap_cont p (ap_merge q H p s1 (ap_merge q0 n s s0 a)) (p & [(l', s', w')]))) in H0.
+         simpl in H0. inversion H0. easy.
+         rewrite(st_eq(merge_ap_cont p (ap_merge q H p s ap_end) (p & [(l', s', w')]))) in H0.
+         simpl in H0. inversion H0. easy.
+Qed.
+
+Lemma pneqq2: forall p q a l l' s s' w w' (H: p <> q),
+  q & [(l, s, w)] = merge_ap_cont p a (p & [(l', s', w')]) ->
+  exists a', w = merge_ap_cont p a' (p & [(l', s', w')]) /\
+  (a = (ap_merge q H l s a') \/ (a = (ap_receive q H l s) /\ a' = ap_end)).
+Proof. intros p q a.
+       induction a; intros.
+       - rewrite(st_eq( merge_ap_cont p (ap_receive q0 n s s0) (p & [(l', s', w')]))) in H0.
+         simpl in H0. inversion H0. subst.
+         exists ap_end. split. rewrite apend_an. easy.
+         right. split. 
+         specialize(proof_irrelevance _ n H); intros. subst. easy. easy.
+       - rewrite(st_eq(merge_ap_cont p (ap_merge q0 n s s0 a) (p & [(l', s', w')]))) in H0.
+         simpl in H0. inversion H0. subst.
+         exists a. split. easy. left.
+         specialize(proof_irrelevance _ n H); intros. subst. easy.
+       - rewrite apend_an in H0. inversion H0. subst. easy.
+Qed.
+
+Fixpoint isInAp {p} (a: Ap p) q: bool :=
+  match a with
+    | ap_merge q' H l s a' => eqb q' q || isInAp a' q
+    | ap_receive q' H l s  => eqb q' q
+    | _                   => false
+  end.
+
+Lemma isInAp_dec: forall {p} (a: Ap p) q, isInAp a q = true \/ isInAp a q = false.
+Proof. intros p a.
+       induction a; intros.
+       - simpl.
+         case_eq(eqb q q0); intros; [left; easy | right; easy].
+         simpl.
+         case_eq(eqb q q0); intros.
+         + rewrite eqb_eq in H. subst.
+           left. easy.
+         + specialize(IHa q0).
+           destruct IHa as [IHa | IHa].
+           -- left. easy.
+           -- right. easy.
+        - simpl. right. easy.
+Qed.
+
+Lemma pRevq: forall p a q l s w,
+  p <> q ->
+  isInAp a q ->
+  exists a' l' s' w',
+  merge_ap_cont p a (p & [(l, s, w)]) = merge_ap_cont q a' (q & [(l', s', w')]).
+Proof. intros p a.
+       induction a; intros.
+       - simpl in H0.
+         apply eqb_eq in H0. subst.
+         rewrite(st_eq(merge_ap_cont p (ap_receive q0 n s s0) (p & [(l, s1, w)]))).
+         simpl.
+         exists ap_end. exists s. exists s0. exists (p & [(l, s1, w)]).
+         rewrite apend_an. easy.
+       - simpl in H0.
+         Search orb.
+         apply Bool.orb_true_iff in H0.
+         destruct H0 as [H0 | H0].
+         + apply eqb_eq in H0. subst.
+           rewrite(st_eq( merge_ap_cont p (ap_merge q0 n s s0 a) (p & [(l, s1, w)]))).
+           simpl. 
+           exists ap_end. exists s. exists s0.
+           exists (merge_ap_cont p a (p & [(l, s1, w)])).
+           rewrite apend_an. easy.
+           
+           rewrite(st_eq(merge_ap_cont p (ap_merge q n s s0 a) (p & [(l, s1, w)]))).
+           simpl.
+           specialize(IHa q0 l s1 w H H0).
+           destruct IHa as (a',(l',(s',(w',IHa)))).
+           rewrite IHa.
+           case_eq(eqb q0 q); intros.
+           -- apply eqb_eq in H1. subst.
+              exists ap_end. exists s. exists s0.
+              exists ( merge_ap_cont q a' (q & [(l', s', w')])).
+              rewrite apend_an. easy.
+           -- apply eqb_neq in H1.
+              exists (ap_merge q H1 s s0 a').
+              exists l'. exists s'. exists w'.
+              rewrite(st_eq(merge_ap_cont q0 (ap_merge q H1 s s0 a') (q0 & [(l', s', w')]))).
+              simpl. easy.
+        - simpl in H0. easy.
+Qed.
+
+Lemma helperRecv:
+  forall a b c r,
+  a ~< b ->
+  b ~< c ->
+  (forall x y z : st, x ~< y -> y ~< z -> r x z) ->
+  paco2 refinementR2 r a c.
+Proof. intros.
+       pfold.
+       red in H, H0.
+       pinversion H.
+       - subst. 
+         pinversion H0.
+         + subst.
+         case_eq (String.eqb p0 p); intros.
+         ++ rewrite eqb_eq in H9. subst.
+            pose proof H5 as H5A.
+            rewrite <- meqAp in H5, H5A.
+            specialize(ApApeqInvAnd p (ApnA2 p a0 n) l l0 s' s0 w' w0); intros HR.
+            symmetry in H5.
+            apply HR in H5.
+            specialize (ApApeqInv p ap_end (ApnA2 p a0 n) l0 l s0 s' w0 w'); intros.
+            rewrite apend_an in H9.
+            apply H9 in H5A. inversion H5A. subst.
+            constructor.
+            admit.
+            rewrite <- meqAp in H3.
+            rewrite H5 in H3.
+            rewrite apend_an in H3.
+            right. apply H1 with (y := w'). easy. easy.
+            admit.
+         ++ rewrite eqb_neq in H9.
+            rename p0 into q.
+            rewrite <- meqAp in H5.
+            assert(p <> q) by easy.
+            apply pneqq2 with (H := H10) in H5.
+            destruct H5 as (a',(Hw0,H5)).
+            destruct H5 as [H5 | H5].
+ 
+            rewrite <- meqAp.
+            rewrite <- meqAp in H3, H7, H8, H4.
+            specialize(isInAp_dec (ApnA2 q a n0) p); intros HLEM.
+            destruct HLEM as [HL| HL].
+            specialize(pRevq q (ApnA2 q a n0) p l0 s'0 w'0 H9 HL); intro HS.
+            destruct HS as (a1,(l1,(s1,(w1,HS)))).
+            rewrite HS.
+Admitted.
+
+Lemma endAp: forall p a l s w, end = merge_ap_cont p a (p & [(l, s, w)]) -> False.
+Proof. intros p a.
+       case_eq a; intros.
+       - rewrite(st_eq(merge_ap_cont p (ap_receive q n s s0) (p & [(l, s1, w)]))) in H0.
+         simpl in H0. easy.
+       - rewrite(st_eq(merge_ap_cont p (ap_merge q n s s0 a0) (p & [(l, s1, w)]))) in H0.
+         simpl in H0. easy.
+       - rewrite apend_an in H0. easy.
+Qed.
+
+Lemma refTrans: Transitive (refinement2).
+Proof. red. pcofix CIH.
+       intros x y z Ha Hb.
+       pinversion Ha. subst.
+       pinversion Hb. subst.
+(*     + punfold H0. punfold H4.
+         pfold. *)
+         case_eq (String.eqb p0 p); intros.
+         ++ rewrite eqb_eq in H6. subst.
+            punfold H0. punfold H4.
+            pfold.
+            pose proof H2 as H2A.
+            rewrite <- meqAp in H2.
+            specialize(ApApeqInvAnd p (ApnA2 p a n) l l0 s' s0 w' w0); intros HR.
+            symmetry in H2.
+            apply HR in H2.
+            rewrite <- meqAp in H0.
+            rewrite H2 in H0. rewrite apend_an in H0.
+            
+            rewrite <- meqAp in H2A.
+            specialize(@ApApeqInv p ap_end (ApnA2 p a n) l0 l s0 s' w0 w'); intros HRA.
+            rewrite apend_an in HRA.
+            apply HRA in H2A.
+            inversion H2A. subst.
+            constructor.
+            admit.
+            * right. apply CIH with (y := w').
+              unfold refinement. pfold. easy.
+              pfold. easy.
+            * rewrite <- meqAp in H1.
+              rewrite H2 in H1. rewrite apend_an in H1.
+              unfold act_eq. intros. split.
+              intros. apply H5. apply H1. easy.
+              intros. apply H1. apply H5. easy.
+              apply refinementR2_mon.
+              apply refinementR2_mon.
+         ++ rewrite eqb_neq in H6.
+            rename p0 into q.
+            rewrite <- meqAp2 in H2.
+            assert(p <> q) by easy.
+            specialize (pneqq2 p q (ApnA p a n) l0 l s0 s' w0 w' H7 H2); intros.
+            destruct H8 as (a',(Hw0,H8)).
+            destruct H8.
+            rewrite <- meqAp2 in H0, H1, H4.
+            rewrite H8 in H0.
+            rewrite(st_eq((merge_ap_cont p (ap_merge q H7 l0 s0 a') w'))) in H0.
+            simpl in H0. rewrite <- meqAp2.
+            rewrite <- meqAp2 in H5.
+            assert(paco2 refinementR2 bot2 (p & [(l, s, w)]) (q & [(l0, s0, merge_ap_cont p a' (p & [(l, s', w')]))])).
+            { pfold.
+              assert((q & [(l0, s0, merge_ap_cont p a' (p & [(l, s', w')]))]) = merge_ap_cont p (ap_merge q H7 l0 s0 a') (p & [(l, s', w')])).
+              { rewrite(st_eq(merge_ap_cont p (ap_merge q H7 l0 s0 a') (p & [(l, s', w')]))). simpl. easy. }
+              rewrite H9.
+              specialize(ref2_a  (upaco2 refinementR2 bot2) w w' p l s s' (ap_merge q H7 l0 s0 a') 1); intro HR.
+              simpl in HR. apply HR.
+              easy.
+              left.
+              rewrite(st_eq((merge_ap_cont p (ap_merge q H7 l0 s0 a') w'))).
+              simpl. easy.
+              rewrite H8 in H1. easy.
+            }
+            rewrite <- Hw0 in H9.
+            assert(paco2 refinementR2 bot2 (q & [(l0, s0, w0)])
+                  (merge_ap_cont q (ApnA q a0 n0) (q & [(l0, s'0, w'0)]))).
+            { pfold. 
+              specialize(ref2_a (upaco2 refinementR2 bot2) w0 w'0 q l0 s0 s'0 (ApnA q a0 n0) 1); intro HR.
+              simpl in HR.
+              apply HR.
+              easy.
+              left. easy.
+              easy.
+            }
+            pose proof CIH as CIH2.
+            specialize(CIH2 (p & [(l, s, w)]) (q & [(l0, s0, w0)])
+                            (merge_ap_cont q (ApnA q a0 n0) (q & [(l0, s'0, w'0)]))
+                            H9 H10).
+            apply helperRecv with (b := (q & [(l0, s0, w0)])). easy. easy. easy.
+            
+            rewrite <- meqAp2 in H0, H1, H4.
+            destruct H8 as (H8a,H8b).
+            rewrite H8a in H0.
+            rewrite(st_eq((merge_ap_cont p (ap_receive q H7 l0 s0) w'))) in H0.
+            simpl in H0.
+            rewrite <- meqAp2.
+            rewrite <- meqAp2 in H5.
+            rewrite Hw0 in H4.
+            assert(paco2 refinementR2 bot2 (p & [(l, s, w)]) (q & [(l0, s0, (p & [(l, s', w')]))])).
+            { pfold.
+              assert((q & [(l0, s0, p & [(l, s', w')])])= merge_ap_cont p (ApnA p a n ) (p & [(l, s', w')])).
+              { rewrite(st_eq(merge_ap_cont p (ApnA p a n) (p & [(l, s', w')]))). rewrite H8a. simpl. easy. }
+              rewrite H8.
+              specialize(ref2_a  (upaco2 refinementR2 bot2) w w' p l s s' (ApnA p a n) 1); intro HR.
+              simpl in HR. apply HR.
+              easy.
+              left.
+              rewrite(st_eq((merge_ap_cont p (ApnA p a n) w'))). rewrite H8a.
+              simpl. easy. easy.
+            }
+            assert(paco2 refinementR2 bot2 (q & [(l0, s0, p & [(l, s', w')])]) (merge_ap_cont q (ApnA q a0 n0) (q & [(l0, s'0, w'0)]))).
+            { pfold.
+              specialize(ref2_a (upaco2 refinementR2 bot2) (p & [(l, s', w')]) w'0 q l0 s0 s'0 (ApnA q a0 n0) 1); intro HR.
+              simpl in HR. apply HR.
+              easy.
+              left.
+              rewrite H8b in H4.
+              rewrite apend_an in H4. easy.
+              rewrite Hw0 H8b in H5.
+              rewrite apend_an in H5. easy.
+            } 
+            pose proof CIH as CIH2.
+            specialize(CIH2 (p & [(l, s, w)]) (q & [(l0, s0, p & [(l, s', w')])])
+                            (merge_ap_cont q (ApnA q a0 n0) (q & [(l0, s'0, w'0)]))
+                            H8 H9).
+            apply helperRecv with (b := (q & [(l0, s0, p & [(l, s', w')])])). easy. easy. easy.
+        
+        (*recv - send case*)
+        subst.
+        symmetry in H2.
+        apply case11 in H2. easy.
+        (*recv - end case*)
+        subst.
+        rewrite <- meqAp2 in H3.
+        apply endAp in H3. easy.
+        
+        apply refinementR2_mon.
+        
+        subst.
+       pinversion Hb. subst.
+       (*send - recv case*)
+       - admit. (*contradicts H2*)
+       
+       subst.
+       - admit.
+       
+       subst.
+       - admit.
+        apply refinementR2_mon.
+        
+        subst. pinversion Hb.
+        pfold. constructor.
+        apply refinementR2_mon.
+        apply refinementR2_mon.
+Admitted.
+
 
