subtyping/refinement.v
@@ -70,5 +70,6 @@ Proof. unfold monotone2.
        - constructor.
 Qed.
 
+
 #[export]
 Declare Instance Ref_Trans: Transitive (refinement).
